Move external path functions to a separate file

fstar/new/MLS.TreeSync.ParentHash.fst
@@ -35,7 +35,7 @@ let ps_parent_hash_input =
   })
   (fun x -> (|x.phin_public_key, (|x.phin_parent_hash, x.phin_original_child_resolution|)|))
 
-val compute_parent_hash_treekem: #cs:ciphersuite -> #l:nat -> #n:tree_size l -> hpke_public_key cs -> bytes -> treekem cs l n -> list (hpke_public_key cs) -> result (lbytes (hash_length cs))
+val compute_parent_hash_treekem: #cs:ciphersuite -> #l:nat -> #n:tree_size l -> hpke_public_key_nt -> bytes -> treekem cs l n -> list (hpke_public_key cs) -> result (lbytes (hash_length cs))
 let compute_parent_hash_treekem #cs #l #n public_key parent_hash sibling forbidden_public_keys =
   let sibling_resolution = tree_resolution sibling in
   let original_child_resolution = List.Tot.filter (fun pk ->
@@ -56,11 +56,19 @@ let compute_parent_hash_treekem #cs #l #n public_key parent_hash sibling forbidd
     }))
   )
 
+val get_public_key_from_content: bytes -> result hpke_public_key_nt
+let get_public_key_from_content content =
+  let open MLS.NetworkBinder in
+  content <-- from_option "get_public_key_from_content: Couldn't parse node content"
+    ((ps_to_pse ps_node_package_content).parse_exact content);
+  return content.npc_public_key
+
 //TODO possible performance optimisation: no need to convert root from treesync to treekem: we only need to convert its content
-val compute_parent_hash_from_sibling: #l:nat -> #ls:nat -> #n:tree_size l -> #ns:tree_size ls -> cs:ciphersuite -> hpke_public_key cs -> bytes -> nat -> treesync l n -> nat -> treesync ls ns -> result (lbytes (hash_length cs))
-let compute_parent_hash_from_sibling #l #ls #n #ns cs public_key parent_parent_hash nb_left_leaves_root root nb_left_leaves_sibling sibling =
+val compute_parent_hash_from_sibling: #l:nat -> #ls:nat -> #n:tree_size l -> #ns:tree_size ls -> cs:ciphersuite -> content:bytes -> parent_parent_hash:bytes -> nat -> treesync l n -> nat -> treesync ls ns -> result (lbytes (hash_length cs))
+let compute_parent_hash_from_sibling #l #ls #n #ns cs content parent_parent_hash nb_left_leaves_root root nb_left_leaves_sibling sibling =
   root_kem <-- treesync_to_treekem_aux cs nb_left_leaves_root root;
   sibling_kem <-- treesync_to_treekem_aux cs nb_left_leaves_sibling sibling;
+  public_key <-- get_public_key_from_content content;
   root_kem_onp <-- (
     match root_kem with
     | TNode root_onp _ _ ->
@@ -76,8 +84,8 @@ let compute_parent_hash_from_sibling #l #ls #n #ns cs public_key parent_parent_h
   in
   compute_parent_hash_treekem public_key parent_parent_hash sibling_kem forbidden_keys
 
-val compute_parent_hash_from_dir: #l:nat -> #n:tree_size l -> cs:ciphersuite -> hpke_public_key cs -> bytes -> nat -> treesync l n -> direction -> result (lbytes (hash_length cs))
-let compute_parent_hash_from_dir #l #n cs public_key parent_parent_hash nb_left_leaves root dir =
+val compute_parent_hash_from_dir: #l:nat -> #n:tree_size l -> cs:ciphersuite -> content:bytes -> parent_parent_hash:bytes -> nat -> treesync l n -> direction -> result (lbytes (hash_length cs))
+let compute_parent_hash_from_dir #l #n cs content parent_parent_hash nb_left_leaves root dir =
   match root with
   | TNode _ left right ->
     let (_, sibling) = order_subtrees dir (left, right) in
@@ -87,33 +95,6 @@ let compute_parent_hash_from_dir #l #n cs public_key parent_parent_hash nb_left_
       else
         nb_left_leaves
     in
-    compute_parent_hash_from_sibling cs public_key parent_parent_hash nb_left_leaves root nb_left_leaves_sibling sibling
+    compute_parent_hash_from_sibling cs content parent_parent_hash nb_left_leaves root nb_left_leaves_sibling sibling
   | _ -> internal_failure "compute_parent_hash_from_dir: `root` must be an internal node"
 
-
-//TODO: this function has bad complexity (because some subtrees are converted a lot of time)
-//Do we care?
-val external_pathsync_to_pathsync_aux: #l:nat -> #n:tree_size l -> #i:leaf_index n -> cs:ciphersuite -> bytes -> nat -> treesync l n -> external_pathsync l n i -> result (pathsync l n i)
-let rec external_pathsync_to_pathsync_aux #l #n #i cs parent_parent_hash nb_left_leaves t p =
-  match t, p with
-  | _, PLeaf lp ->
-    //TODO check that the parent hash in lp is correct
-    return (PLeaf (Some lp))
-  | TSkip _ t', PSkip _ p' ->
-    result <-- external_pathsync_to_pathsync_aux cs parent_parent_hash nb_left_leaves t' p';
-    return (PSkip _ result)
-  | TNode _ left right, PNode np p_next ->
-    let (|dir, next_i|) = child_index l i in
-    let (child, sibling) = order_subtrees dir (left, right) in
-    let child_nb_left_leaves = if dir = Left then nb_left_leaves else nb_left_leaves + (pow2 (l-1)) in
-    public_key <-- (
-      kem_node_package <-- treesync_to_treekem_node_package cs nb_left_leaves np;
-      return kem_node_package.kp_public_key
-    );
-    parent_hash <-- compute_parent_hash_from_dir cs public_key parent_parent_hash nb_left_leaves t dir;
-    result_p_next <-- external_pathsync_to_pathsync_aux cs parent_hash child_nb_left_leaves child p_next;
-    return (PNode (Some ({np with np_parent_hash = parent_parent_hash;})) result_p_next)
-
-val external_pathsync_to_pathsync: #l:nat -> #n:tree_size l -> #i:leaf_index n -> cs:ciphersuite -> treesync l n -> external_pathsync l n i -> result (pathsync l n i)
-let external_pathsync_to_pathsync #l #n #i cs t p =
-  external_pathsync_to_pathsync_aux cs bytes_empty 0 t p
