fstar/new/MLS.Test.TreeKEM.fst
@@ -7,6 +7,7 @@ open MLS.Test.Utils
 open MLS.Tree
 open MLS.TreeSync.Types
 open MLS.TreeSync.ParentHash
+open MLS.TreeSync.ExternalPath
 open MLS.TreeSync
 open MLS.TreeSync.Hash
 open MLS.TreeKEM
