fstar/new/MLS.TreeSync.ExternalPath.fst
@@ -1,0 +1,32 @@
+module MLS.TreeSync.ExternalPath
+
+open Lib.ByteSequence
+open MLS.Tree
+open MLS.Crypto
+open MLS.TreeSync.Types
+open MLS.TreeSync.ParentHash
+open MLS.Result
+
+//TODO: this function has bad complexity (because some subtrees are converted a lot of time)
+//Do we care?
+val external_pathsync_to_pathsync_aux: #l:nat -> #n:tree_size l -> #i:leaf_index n -> cs:ciphersuite -> bytes -> nat -> treesync l n -> external_pathsync l n i -> result (pathsync l n i)
+let rec external_pathsync_to_pathsync_aux #l #n #i cs parent_parent_hash nb_left_leaves t p =
+  match t, p with
+  | _, PLeaf lp ->
+    //TODO check that the parent hash in lp is correct
+    return (PLeaf (Some lp))
+  | TSkip _ t', PSkip _ p' ->
+    result <-- external_pathsync_to_pathsync_aux cs parent_parent_hash nb_left_leaves t' p';
+    return (PSkip _ result)
+  | TNode _ left right, PNode np p_next ->
+    let (|dir, next_i|) = child_index l i in
+    let (child, sibling) = order_subtrees dir (left, right) in
+    let child_nb_left_leaves = if dir = Left then nb_left_leaves else nb_left_leaves + (pow2 (l-1)) in
+    parent_hash <-- compute_parent_hash_from_dir cs np.np_content parent_parent_hash nb_left_leaves t dir;
+    result_p_next <-- external_pathsync_to_pathsync_aux cs parent_hash child_nb_left_leaves child p_next;
+    return (PNode (Some ({np with np_parent_hash = parent_parent_hash;})) result_p_next)
+
+val external_pathsync_to_pathsync: #l:nat -> #n:tree_size l -> #i:leaf_index n -> cs:ciphersuite -> treesync l n -> external_pathsync l n i -> result (pathsync l n i)
+let external_pathsync_to_pathsync #l #n #i cs t p =
+  external_pathsync_to_pathsync_aux cs bytes_empty 0 t p
+
